TM/Code/MatchList.v
@@ -1,0 +1,353 @@
+(* Product destruct and construction *)
+
+Require Import TM.Code.CodeTM.
+Require Import TM.Basic.Mono TM.Basic.Nop TM.Basic.Multi.
+Require Import TM.Combinators.Combinators.
+Require Import TM.LiftMN TM.LiftSigmaTau.
+Require Import TM.Compound.TMTac.
+Require Import TM.Compound.CopySymbols TM.Compound.MoveToSymbol.
+Require Import TM.Code.Copy.
+
+Section MatchList.
+
+  (*
+  Section Test.
+
+    Let f {tau : Type} (x : (bool + (tau + (bool + tau)))) : (bool + tau) :=
+      match x with
+      | inl x => inl x
+      | inr (inl y) => inr y
+      | inr (inr (inl y)) => inl y
+      | inr (inr (inr y)) => inr y
+      end.
+
+    Let g {tau : Type} (x: bool + tau) : option (bool + (tau + (bool + tau))) :=
+      match x with
+      | inl y => Some (inl y)
+      | inr y => Some (inr (inl y))
+      end.
+
+    Section Test.
+      (* The encoding of a list is a concatenation of encoding of options *)
+
+      Compute encode [].
+      Compute encode None.
+      Compute encode [1;2;3] : list (bool + bool).
+      Compute encode (true, (1, [2;3])).
+      Compute encode (true, (1, [2;3])) : list (bool + (bool + (bool + bool))).
+      Compute encode (true, (tt, [tt;tt])) : list (bool + (unit + (bool + unit))).
+      Compute map f (encode (true, (tt, [tt;tt])) : list (bool + (unit + (bool + unit)))).
+
+      Goal encode [1;2;3] = encode (Some 1) ++ encode (Some 2) ++ encode (Some 3) ++ encode None.
+      Proof. cbn. trivial. Qed.
+
+      Goal encode [1;2;3] = map f (encode (true, (1, [2; 3]))).
+      Proof. cbn. trivial. Qed.
+
+      Goal encode [tt;tt;tt] = map f (encode (true, (tt, [tt;tt]))).
+      Proof. cbn. trivial. Qed.
+      
+    End Test.
+
+    Variable X : Type.
+    Variable (sigX : finType).
+    Hypothesis (codX : codeable sigX X).
+
+    Lemma encode_f_cons (x : X) (xs : list X) :
+      map f (encode (true, (x, xs))) = encode (x :: xs).
+    Proof.
+      cbn. f_equal. repeat rewrite !map_app, !List.map_map. cbn. f_equal.
+      erewrite map_ext.
+      - eapply map_id.
+      - intuition.
+    Qed.
+
+    Lemma retr' (tau : Type) : retract (@f tau) (@g tau).
+    Proof.
+      hnf. intros x. intuition; cbn; auto.
+    Abort.
+
+  End Test.
+   *)
+
+
+  Variable X : Type.
+  Variable (sigX : finType).
+  Hypothesis (codX : codeable sigX X).
+
+  Definition M1 : { M : mTM (bool + sigX)^+ 1 & states M -> bool } :=
+    MATCH (Read_char _)
+          (fun o => match o with
+                 | Some (inr (inl true))  => mono_Nop _ true  (* inl *)
+                 | Some (inr (inl false)) => mono_Nop _ false (* inr *)
+                 | _ => mono_Nop _ true (* invalid input *)
+                 end).
+
+  Let R1 : Rel (tapes (bool+sigX)^+ 1) (bool * tapes (bool+sigX)^+ 1) :=
+    Mk_R_p (
+        (if? (fun (tin tout : tape (bool+sigX)^+) =>
+                   forall (lst : list X),
+                     tin ≂ lst ->
+                     exists (head : X) (tail : list X),
+                       lst = head :: tail)
+              ! (fun (tin tout : tape (bool+sigX)^+) =>
+                   forall (lst : list X),
+                     tin ≂ lst ->
+                     lst = nil)
+        ) ∩ ignoreParam (@IdR _)). 
+
+  Lemma M1_Sem : M1 ⊨c(5) R1.
+  Proof.
+    eapply RealiseIn_monotone.
+    {
+      eapply Match_RealiseIn. cbn. eapply read_char_sem.
+      instantiate (2 := fun o : option (bool + sigX)^+ =>
+                          match o with Some (inr (inl true)) => _ | Some (inr (inl false)) => _ | _ => _ end).
+      cbn. intros [ s | ]; cbn.
+      - destruct s as [ start | s]; cbn.
+        + eapply RealiseIn_monotone'. eapply mono_Nop_Sem. omega.
+        + destruct s as [cons | xy]; swap 1 2; cbn.
+          * eapply RealiseIn_monotone'. eapply mono_Nop_Sem. omega.
+          * destruct cons; cbn; eapply mono_Nop_Sem.
+      - eapply RealiseIn_monotone'. eapply mono_Nop_Sem. omega.
+    }
+    { cbn. omega. }
+    {
+      subst R1.
+      intros tin (yout&tout) H. destruct H as (H1&(t&(H2&H3)&H4)); hnf in *. subst.
+      split.
+      {
+        destruct_tapes; cbn in *.
+        destruct h; cbn in *; TMSimp; eauto. destruct (map _) in H0; cbn in H0; congruence.
+        destruct e; swap 1 2; cbn in *; TMSimp.
+        - destruct s; swap 1 2; cbn in *; TMSimp.
+          + destruct lst; cbn in *; inv H0.
+          + destruct b; cbn in *; TMSimp cbn in *; unfold encode_list in *.
+            * destruct lst; TMSimp cbn in *. eauto.
+            * destruct lst; TMSimp cbn in *. eexists; split; eauto.
+        - destruct lst; cbn in *; inv H0; eauto.
+      }
+      {
+        destruct_tapes; cbn in *.
+        destruct h; cbn in *; TMSimp; eauto. destruct e; cbn in *; TMSimp; auto.
+        destruct s; cbn in *; TMSimp; auto.
+        destruct b; cbn in *; TMSimp cbn in *; auto.
+      }
+    }
+  Qed.
+
+  Definition stop_X' :=
+    fun (x : (bool+sigX)^+) =>
+      match x with
+      | inr (inr x) => false
+      | _ => true (* Stop at the next constructor or start/end symbol *)
+      end.
+
+  (* Copy the head encoding to tape 1 and set new start token on tape 0. *)
+  Let M2 : { M : mTM (bool+sigX)^+ 2 & states M -> unit } :=
+    Inject (Move _ R tt) [|Fin.F1|];;
+    CopySymbols stop_X' id;;
+    Inject (
+      Move _ L tt;;
+      WriteMove (Some (inl START), R) tt (* write the start symbol *)
+    ) [|Fin.F1|].
+
+  (* Copy the symbols from tape 0 to tape 1, finish tape 0 but not don't initialise tape 1 *)
+  Let R2 : Rel (tapes (bool + sigX)^+ 2) (unit * tapes (bool + sigX)^+ 2) :=
+    ignoreParam (
+        fun (tin tout : tapes (bool + sigX)^+ 2) =>
+          forall (head : X) (tail : list X),
+            tin [@Fin.F1] ≂ head :: tail ->
+            tout[@Fin.F1] ≂ tail /\
+            left (tout[@Fin.FS Fin.F1]) =
+            rev (map inr (map inr (encode head : list sigX))) ++ left (tin[@Fin.FS Fin.F1])
+      ).
+
+
+  Lemma CopySymbols_cons_first (head : X) (tail : list X) tltr tl' tr' rs' :
+    (tl', tr') = CopySymbols_Fun stop_X' id tltr ->
+    tape_local (fst tltr) = map inr (map inr (encode head)) ++ map inr (encode tail) ++ (inl STOP :: rs') ->
+    tape_local (tl') = map inr (encode tail) ++ (inl STOP :: rs').
+  Proof.
+    intros. destruct tail as [ | ctail tail'] eqn:E1; cbn in *.
+    - refine (CopySymbols_pair_first _ _ H0 H).
+      + rewrite List.map_map. intros x (? & <- & ?) % in_map_iff. cbn. trivial.
+      + cbn. trivial.
+    - refine (CopySymbols_pair_first _ _ H0 H).
+      + rewrite List.map_map. intros x (? & <- & ?) % in_map_iff. cbn. trivial.
+      + cbn. trivial.
+  Qed.
+
+  Lemma CopySymbols_cons_second (head : X) (tail : list X) tltr tl' tr' rs' :
+    (tl', tr') = CopySymbols_Fun stop_X' id tltr ->
+    tape_local (fst tltr) = map inr (map inr (encode head)) ++ map inr (encode tail) ++ (inl STOP :: rs') ->
+    left tr' = map inr (map inr (rev (encode head : list sigX))) ++ left (snd tltr).
+  Proof.
+    intros. rewrite !map_rev. destruct tail as [ | ctail tail'] eqn:E1; cbn in *.
+    - refine (CopySymbols_pair_second _ _ H0 H).
+      + rewrite List.map_map. intros x (? & <- & ?) % in_map_iff. cbn. trivial.
+      + cbn. trivial.
+    - refine (CopySymbols_pair_second _ _ H0 H).
+      + rewrite List.map_map. intros x (? & <- & ?) % in_map_iff. cbn. trivial.
+      + cbn. trivial.
+  Qed.
+  
+  Lemma M2_WRealise : M2 ⊫ R2.
+  Proof.
+    subst M2 R1 R2.
+    eapply WRealise_monotone.
+    {
+      do 2 try eapply Seq_WRealise.
+      all: try (eapply Inject_WRealise; [vector_dupfree| ]).
+      3: do 1 eapply Seq_WRealise.
+      all: try (eapply Realise_WRealise, RealiseIn_Realise;
+                first [ eapply Move_Sem | eapply WriteMove_Sem | eapply Write_Sem ]).
+      - eapply CopySymbols_WRealise.
+    }
+    {
+      hnf. intros. hnf. destruct y. intros head tail.
+      TMSimp repeat progress simpl_not_in || cbn [Vector.nth] in *. destruct u.
+      destruct h1; cbn in *; inv H0; [ do 2 destruct (map _); cbn in H3; congruence | inv H3]. clear H1. 
+      split.
+      - 
+        epose proof CopySymbols_cons_first H (head := head) (tail := tail) (rs' := x1) as L1. cbn in *.
+        spec_assert L1.
+        {
+          destruct (encode head); cbn.
+          - destruct (encode_list codX tail); cbn; auto.
+          - f_equal. now rewrite !List.map_app, <- app_assoc.
+        }
+        hnf.
+        do 2 eexists; split; cbn.
+        + eapply tape_match_left_right.
+        + erewrite <- L1. destruct h2; cbn in *; auto. destruct (encode_list _); cbn in *; congruence. destruct l; cbn; auto.
+      -
+        epose proof CopySymbols_cons_second H (head := head) (tail := tail) (rs' := x1) as L1. cbn in *.
+        spec_assert L1.
+        {
+          destruct (encode head); cbn.
+          - destruct (encode_list codX tail); cbn; auto.
+          - f_equal. now rewrite !List.map_app, <- app_assoc.
+        }
+        hnf. now rewrite !map_rev, List.map_map in *.
+    }
+  Qed.
+
+  Let M3 : { M : mTM (bool+sigX)^+ 2 & states M -> unit } :=
+    Inject (WriteMove (Some (inl START), R) tt) [|Fin.FS Fin.F1|];;
+    M2;;
+    Inject (
+      WriteMove (Some (inl STOP), L) tt;;
+      MoveToSymbol_L stop_X';;
+      Move _ R tt
+    ) [|Fin.FS Fin.F1|].
+
+  Let R3 : Rel (tapes (bool+sigX)^+ 2) (unit * tapes (bool+sigX)^+ 2) :=
+    ignoreParam (
+        fun (tin tout : tapes (bool+sigX)^+ 2) =>
+          forall (head : X) (tail : list X),
+            tin [@Fin.F1] ≂ head :: tail ->
+            tout[@Fin.F1] ≂ tail /\
+            tout[@Fin.FS Fin.F1] ≂ head
+      ).
+
+
+  Lemma M3_WRealise : M3 ⊫ R3.
+  Proof.
+    eapply WRealise_monotone.
+    {
+      do 2 try eapply Seq_WRealise.
+      all: try (eapply Inject_WRealise; [vector_dupfree| ]).
+      3: repeat eapply Seq_WRealise.
+      all: try (eapply Realise_WRealise, RealiseIn_Realise;
+                first [ eapply Move_Sem | eapply WriteMove_Sem | eapply Write_Sem ]).
+      - eapply M2_WRealise.
+      - eapply MoveToSymbol_L_WRealise.
+    }
+    {
+      subst R1 M2 R2 M3 R3. hnf. intros. hnf. destruct y. intros head tail.
+      TMSimp repeat progress simpl_not_in || cbn [Vector.nth] in *. destruct u.
+      destruct h3; cbn in *; inv H0; [destruct (encode _); cbn in H3; congruence | inv H3]. clear H1.
+      specialize (H head tail). spec_assert H by (hnf; do 2 eexists; hnf; split; cbn; eauto). destruct H as (H1&H1').
+      split; eauto. hnf; unfold tape_encodes_r; cbn in *. clear b H2 H1.
+      rewrite tape_match_left_right in *. unfold finType_CS in *; rewrite H1' in *.
+
+      assert (tape_local_l (tape_move_mono h4 (Some (inl STOP), L)) =
+              rev (map inr (map inr (encode head))) ++ inl START :: left h2) as L1.
+      {
+        repeat ( rewrite <- !app_assoc in *; cbn in * ).
+        destruct h4; cbn in *; try congruence. subst. apply tape_match_symbols_tape_local_l.
+      }
+
+      epose proof (MoveToSymbol_L_left (stop := stop_X') _ _ L1) as (L2&L3).
+      epose proof (MoveToSymbol_L_right (stop := stop_X') _ _ L1) as L4.
+
+      cbn in *. rewrite H1' in *.
+      progress unfold finType_CS in *.
+      do 2 eexists; hnf; split; cbn in *; eauto.
+      + erewrite tape_left_move_right; eauto.
+      + erewrite tape_local_move_right; eauto.
+        eapply tape_local_iff. do 2 eexists. split; eauto. split.
+        eapply L3. rewrite L4. cbn. rewrite tape_match_symbols_right. cbn. now rewrite rev_involutive.
+
+      Unshelve.
+      2,3,4: cbn; trivial.
+      1,2: intros x; rewrite !List.map_map, <- map_rev; intros (? & <- & ?) % in_map_iff; cbn; trivial.
+    }
+  Qed.
+
+  Definition MatchList : { M : mTM (bool+sigX)^+ 2 & states M -> bool } :=
+    If (Inject M1 [|Fin.F1|])
+       (M3;; Nop _ _ true)
+       (Nop _ _ false).
+
+  Definition MatchList_Rel : Rel (tapes (bool+sigX)^+ 2) (bool * tapes (bool+sigX)^+ 2) :=
+    (if? (fun (tin tout : tapes (bool+sigX)^+ 2) =>
+          forall (lst : list X),
+            tin[@Fin.F1] ≂ lst ->
+            exists (head : X) (tail : list X),
+              lst = head :: tail /\
+              tout[@Fin.F1] ≂ tail /\
+              tout[@Fin.FS Fin.F1] ≂ head)
+       ! (fun (tin tout : tapes (bool+sigX)^+ 2) =>
+            forall (lst : list X),
+            tin[@Fin.F1] ≂ lst ->
+              lst = nil /\
+              tout[@Fin.F1] ≂ nil)).
+
+  Lemma MatchList_Sem :
+    MatchList ⊫ MatchList_Rel.
+  Proof.
+    eapply WRealise_monotone.
+    {
+      unfold MatchList. eapply If_WRealsie.
+      - eapply Inject_WRealise. vector_dupfree. eapply Realise_WRealise, RealiseIn_Realise. eapply M1_Sem.
+      - eapply Seq_WRealise.
+        + eapply M3_WRealise.
+        + eapply Realise_WRealise, RealiseIn_Realise. eapply Nop_total.
+      - eapply Realise_WRealise, RealiseIn_Realise. eapply Nop_total.
+    }
+    {
+      subst R1 M2 R2 M3 R3. cbn.
+      TMSimp repeat progress simpl_not_in || cbn [Vector.nth] in *.
+      destruct b, H; TMSimp repeat progress simpl_not_in || cbn [Vector.nth] in *.
+      - specialize (H lst). spec_assert H as (head&tail&->) by (do 2 eexists; split; cbn; eauto).
+        specialize (H1 head tail).
+        spec_assert H1 as (H1&H1').
+        {
+          hnf. do 2 eexists; split; cbn in *; eauto.
+        }
+        do 2 eexists; repeat split; eauto.
+      - auto.
+      - congruence.
+      - assert (lst = nil) as ->.
+        {
+          eapply H. cbn. hnf; do 2 eexists; split; cbn; eauto.
+        }
+        split; eauto. hnf. do 2 eexists; split; cbn in *; eauto.
+    }
+  Qed.
+
+  (* TODO: Termination *)
+
+End MatchList.
