TM/Code/MatchProd.v
@@ -1,0 +1,208 @@
+(* Product destruct and construction *)
+
+Require Import TM.Code.CodeTM.
+Require Import TM.Basic.Mono TM.Basic.Nop TM.Basic.Multi.
+Require Import TM.Combinators.Combinators.
+Require Import TM.LiftMN TM.LiftSigmaTau.
+Require Import TM.Compound.TMTac.
+Require Import TM.Compound.CopySymbols TM.Compound.MoveToSymbol.
+Require Import TM.Code.Copy.
+
+Section Projection.
+
+  Variable X Y : Type.
+  Variable (sigX sigY : finType).
+  Hypothesis (codX : codeable sigX X) (codY : codeable sigY Y).
+
+
+  Definition stop_X :=
+    fun (x : (sigX+sigY)^+) =>
+      match x with
+      | (inr (inl _)) => false
+      | _ => true (* Stop at symbol from Y or halt/stop symbol *)
+      end.
+
+  Definition stop_Y :=
+    fun (x : (sigX+sigY)^+) =>
+      match x with
+        inr (inr _) => false
+      | _ => true (* Stop at symbol from X or halt/stop symbol *)
+      end.
+
+
+  Local Lemma CopySymbols_pair_first' (inputX : list sigX) (inputY : list sigY) tltr tl' tr' rs' :
+    tape_local (fst tltr) = map inr (map inl inputX ++ map inr inputY) ++ (inl STOP :: rs') ->
+    (tl', tr') = CopySymbols_Fun stop_X id tltr ->
+    tape_local (tl') = map inr (map inr inputY) ++ (inl STOP :: rs').
+  Proof.
+    intros. destruct inputY as [ | csy inputY'] eqn:E1; cbn in *.
+    - eapply CopySymbols_pair_first; cbn; eauto.
+      + rewrite app_nil_r. intuition. eapply in_map_iff in H1 as (?&<-& (?&<-&?)%in_map_iff). trivial.
+      + trivial.
+    - eapply CopySymbols_pair_first with (str1 := map inr (map inl inputX)); cbn; eauto.
+      + intros x. rewrite !List.map_map. intros (?&<-&?) % in_map_iff. cbn. trivial.
+      + simpl_list. intuition.
+      + now rewrite map_app, <- app_assoc in H.
+  Qed.
+
+  Local Lemma CopySymbols_pair_first'' (inputX : list sigX) (inputY : list sigY) ls m rs tr tl' tr' rs' :
+    m :: rs = map inr (map inl inputX ++ map inr inputY) ++ inl STOP :: rs' ->
+    (tl', tr') = CopySymbols_Fun stop_X id (midtape ls m rs, tr) ->
+    tape_local tl' = map inr (map inr inputY) ++ inl STOP :: rs'.
+  Proof.
+    intros H1 H2. apply (CopySymbols_pair_first' (tltr := (midtape ls m rs, tr)) ltac:(cbn; eapply H1) H2).
+  Qed.
+
+  Local Lemma CopySymbols_pair_second' (inputX : list sigX) (inputY : list sigY) tltr tl' tr' rs' :
+    tape_local (fst tltr) = map inr (map inl inputX ++ map inr inputY) ++ (inl STOP :: rs') ->
+    (tl', tr') = CopySymbols_Fun stop_X id tltr ->
+    left tr' = map inr (map inl (rev inputX)) ++ left (snd tltr).
+  Proof.
+    intros. rewrite !map_rev. destruct inputY as [ | csy inputY'] eqn:E1; cbn in *.
+    - rewrite app_nil_r in H.
+      eapply CopySymbols_pair_second; cbn; eauto.
+      + intros ? (? & <- & (? & <- & ?) % in_map_iff) % in_map_iff. cbn. trivial.
+      + cbn. trivial.
+    - eapply CopySymbols_pair_second with (str1 := map inr (map inl inputX)); cbn; eauto; swap 2 3.
+      + intros x. rewrite !List.map_map. intros (?&<-&?) % in_map_iff. cbn. trivial.
+      + rewrite map_app, <- app_assoc in H. eapply H.
+      + trivial.
+  Qed.
+  
+  Local Lemma CopySymbols_pair_second'' (inputX : list sigX) (inputY : list sigY) ls m rs tr tl' tr' rs' :
+    m :: rs = map inr (map inl inputX ++ map inr inputY) ++ inl STOP :: rs' ->
+    (tl', tr') = CopySymbols_Fun stop_X id (midtape ls m rs, tr) ->
+    left tr' = map inr (map inl (rev inputX)) ++ left tr.
+  Proof.
+    intros H1 H2. apply (CopySymbols_pair_second' (tltr := (midtape ls m rs, tr)) ltac:(cbn; eapply H1) H2).
+  Qed.
+
+
+  Let M1 : { M : mTM (sigX+sigY)^+ 2 & states M -> unit } :=
+    CopySymbols stop_X id;;
+    Inject (
+      (Move _ L tt);;
+      WriteMove (Some (inl START), R) tt
+    ) [|Fin.F1|].
+
+  
+  (* Copy the symbols from tape 0 to tape 1, finish tape 0 but not don't initialise tape 1 *)
+  Let R1 : Rel (tapes (sigX+sigY)^+ 2) (unit * tapes (sigX+sigY)^+ 2) :=
+    ignoreParam (
+        fun (tin tout : tapes (sigX+sigY)^+ 2) =>
+          forall (xy : X * Y),
+            tin [@Fin.F1] ≂ xy ->
+            tout[@Fin.F1] ≂ snd xy /\
+            left (tout[@Fin.FS Fin.F1]) = rev (map inr (map inl (encode (fst xy)))) ++ left (tin[@Fin.FS Fin.F1])
+      ).
+
+  
+  Local Lemma M1_WRealise : M1 ⊫ R1.
+  Proof.
+    subst M1 R1.
+    eapply WRealise_monotone.
+    {
+      do 1 try eapply Seq_WRealise.
+      all: try (eapply Inject_WRealise; [vector_dupfree| ]).
+      2: eapply Seq_WRealise.
+      all: try (eapply Realise_WRealise, RealiseIn_Realise;
+                first [ eapply Move_Sem | eapply WriteMove_Sem | eapply Write_Sem ]).
+      - eapply CopySymbols_WRealise.
+    }
+    {
+      hnf. intros. hnf. destruct y. intros (inputX, inputY).
+      TMSimp repeat progress simpl_not_in || cbn [Vector.nth] in *. destruct u.
+      destruct h1; cbn in *; inv H0; [ do 2 destruct (encode _); cbn in H2; congruence | ]. clear H1.
+      (*
+      erewrite List.map_app, !List.map_map, <- app_assoc in H3; cbn in H3.
+       *)
+      split.
+      - pose proof CopySymbols_pair_first'' H2 H as L1.
+        destruct h3; cbn in *; try (destruct (encode inputY); cbn in L1; congruence).
+        destruct l; cbn in *.
+        + hnf. do 2 eexists. split; cbn; eauto.
+        + hnf. do 2 eexists. split; cbn; eauto.
+      - pose proof (CopySymbols_pair_second'' H2 H) as ->. now rewrite !map_rev.
+    }
+  Qed.
+  
+  Definition Proj : { M : mTM (sigX+sigY)^+ 2 & states M -> unit } :=
+    Inject (WriteMove (Some (inl START), R) tt) [|Fin.FS Fin.F1|];;
+    M1;;
+    Inject (
+      WriteMove (Some (inl STOP), L) tt;;
+      MoveToSymbol_L stop_X;;
+      Move _ R tt
+    ) [|Fin.FS Fin.F1|].
+
+  
+  Definition Proj_Rel : Rel (tapes (sigX+sigY)^+ 2) (unit * tapes (sigX+sigY)^+ 2) :=
+    ignoreParam (
+        fun (tin tout : tapes (sigX+sigY)^+ 2) =>
+          forall (xy : X * Y),
+            tin [@Fin.F1] ≂ xy ->
+            tout[@Fin.F1] ≂ snd xy /\
+            tout[@Fin.FS Fin.F1] ≂ fst xy
+      ).
+
+  (* Θ (18 + (4+?)*(?+1)*|enocode (fst x)|) *)
+
+  (* TODO: add the above lemmas to Prelim.v bzw. CodeTM.v and add them to the tape database *)
+
+  Lemma Proj_WRealise : Proj ⊫ Proj_Rel.
+  Proof.
+    eapply WRealise_monotone.
+    {
+      unfold Proj. do 2 try eapply Seq_WRealise.
+      all: try (eapply Inject_WRealise; [vector_dupfree| ]).
+      3: repeat eapply Seq_WRealise.
+      all: try (eapply Realise_WRealise, RealiseIn_Realise;
+                first [ eapply Move_Sem | eapply WriteMove_Sem | eapply Write_Sem ]).
+      - eapply M1_WRealise.
+      - eapply MoveToSymbol_L_WRealise.
+    }
+    {
+      hnf. intros. hnf. destruct y. intros (inputX, inputY).
+      TMSimp repeat progress simpl_not_in || cbn [Vector.nth] in *. destruct u.
+      destruct h3; cbn in *; inv H0; [do 2 destruct (encode _); cbn in H3; congruence | ]. clear H1. clear M1 R1. 
+      specialize (H (inputX, inputY)). spec_assert H by (hnf; do 2 eexists; hnf; split; cbn; eauto). destruct H as (H1&H1').
+      split; eauto. hnf; unfold tape_encodes_r; cbn in *. clear b H2 H1 h H3.
+      rewrite tape_match_left_right in *. unfold finType_CS in *; rewrite H1'.
+
+      destruct (encode inputX) as [ | cs cX'] eqn:E1; cbn in *.
+      - do 2 eexists; hnf; split; cbn; hnf; rewrite MoveToSymbol_L_Fun_equation; cbn; eauto.
+      - repeat ( rewrite <- !app_assoc in *; cbn in * ).
+
+        assert (tape_local_l (tape_move_mono h4 (Some (inl STOP), L)) =
+                (rev (map inr (map inl cX')) ++ [inr (inl cs)]) ++ inl START :: left h2) as L1.
+        {
+          repeat ( rewrite <- !app_assoc in *; cbn in * ).
+          destruct h4; cbn in *; try (destruct cX'; cbn in *; congruence). subst. apply tape_match_symbols_tape_local_l.
+        }
+        
+        (* TODO: This is a little mess! *)
+        epose proof MoveToSymbol_L_left (stop := stop_X) _ _ L1 as (L2&L3). Unshelve. all: eauto.
+        Focus 2.
+        rewrite <- !map_rev, List.map_map. intros x [ (?&<-&?) % in_map_iff | [ <- | H]] % in_app_iff; cbn; auto.
+        epose proof MoveToSymbol_L_right (stop := stop_X) _ _ L1 as L4. Unshelve. all: eauto.
+        Focus 2.
+        rewrite <- !map_rev, List.map_map. intros x [ (?&<-&?) % in_map_iff | [ <- | H]] % in_app_iff; cbn; auto.
+        cbn in *. rewrite H1' in *. cbn in *.
+        do 2 eexists; hnf; split; cbn; eauto.
+        + erewrite tape_left_move_right; eauto.
+        + erewrite tape_local_move_right; eauto.
+          eapply tape_local_iff. do 2 eexists. split; eauto. split.
+          eapply L3. unfold finType_CS in *. rewrite L4. cbn.
+          rewrite tape_match_symbols_right. cbn.
+          rewrite rev_app_distr; cbn. rewrite <- !map_rev, rev_involutive. eauto.
+    }
+  Qed.
+
+
+  (* TODO Termination *)
+
+  (* TODO: Konstruktor *)
+  
+
+End Projection.
+
